share/steel/examples/pulse/bug-reports/Global.fst
@@ -1,0 +1,79 @@
+module Global
+open Pulse.Main
+open Pulse.Steel.Wrapper
+module W = Pulse.Steel.Wrapper
+open FStar.Ghost
+open Steel.ST.Util
+open Steel.FractionalPermission
+open Steel.ST.Array
+module A = Steel.ST.Array
+module R = Steel.ST.Reference
+module US = FStar.SizeT
+open Array 
+
+(* mutate global vars that are assumed *)
+
+assume val r : R.ref int
+
+```pulse 
+fn init_global_ref (_:unit) 
+  requires exists v. R.pts_to r full_perm v
+  ensures exists v. R.pts_to r full_perm v
+{
+  r := 0;
+  ()
+}
+```
+
+assume val l : l:US.t{US.v l > 0}
+assume val a : A.array int
+assume val s : s:Ghost.erased (Seq.seq int){Seq.length s = US.v l}
+
+```pulse 
+fn init_global_array (_:unit) 
+  requires A.pts_to a full_perm s
+  ensures exists s_. A.pts_to a full_perm s_
+{
+  (a.(0sz) <- 0);
+  with s_. assert A.pts_to a full_perm s_;
+  ()
+}
+```
+
+(* Initialize global variables by calling Pulse.Steel.Wrapper functions 
+
+Want to initialize global variables using steel wrapper functions
+but they return stt types. 
+
+To do this, we either need to be able to write global vars within Pulse's scope:
+
+```pulse
+let r2 : R.ref int = W.alloc 0
+```
+
+or to be able to extract the underlying type from the stt type in the FStar
+let binding. 
+
+*)
+
+[@@expect_failure]
+(* 
+Returns 
+  stt (R.ref int) emp (fun r -> R.pts_to r full_perm 0)
+Instead of 
+  R.ref int
+*)
+let r2 : R.ref int = W.alloc 0
+
+[@@expect_failure]
+(* 
+Returns 
+  stt (A.array int) 
+      (requires emp)
+      (ensures fun a ->
+        A.pts_to a full_perm (Seq.create (US.v l) 0) `star`
+        pure (A.length a == US.v l /\ A.is_full_array a))
+Instead of
+  A.array int
+*)
+let a2 : A.array int = W.new_array 0 l 
