share/steel/examples/pulse/bug-reports/SpinLock.fst
@@ -5,9 +5,9 @@ open FStar.Ghost
 open Steel.ST.Util
 open Steel.FractionalPermission
 module R = Steel.ST.Reference
+module L = Steel.ST.SpinLock
 #push-options "--ide_id_info_off"
 
-(* this works *)
 ```pulse
 fn lock_ref (r:R.ref int) (#v_:Ghost.erased int)
   requires R.pts_to r full_perm v_
@@ -20,40 +20,19 @@ fn lock_ref (r:R.ref int) (#v_:Ghost.erased int)
 ```
 
 
-(* 
-  pulse fails to instantiate the existential var in
-  the post condition
-*)
-[@@expect_failure]
-```pulse
-fn create_and_lock_ref (_:unit)
-  requires emp
-  returns r:R.ref int
-  ensures exists v. R.pts_to r full_perm v
-{
-  let mut r = 0;
-  let my_lock = new_lock (exists_ (fun v -> R.pts_to r full_perm v));
-  acquire #(exists_ (fun v -> R.pts_to r full_perm v)) my_lock;
-  r
-}
-```
-
-
 let ref_prop (r:R.ref int) : vprop
   = exists_ (fun v -> R.pts_to r full_perm v)
 
-(*
-  pulse fails to unify (ref_prop r) with (R.pts_to r full_perm v_)
-  on line 55
-*)
-[@@expect_failure]
 ```pulse
-fn lock_ref_refactor (r:R.ref int) (#v_:Ghost.erased int)
-  requires R.pts_to r full_perm v_
-  ensures exists v. R.pts_to r full_perm v
+fn lock_ref_refactor (r:R.ref int)
+  requires ref_prop r
+  returns l:L.lock (ref_prop r)
+  ensures emp
 {
   let my_lock = new_lock (ref_prop r);
   acquire #(ref_prop r) my_lock;
-  ()
+  release #(ref_prop r) my_lock;
+  my_lock
 }
 ```
+
